>[!note] $f^{-1} \circ f = I_{X} \quad (f:X \rightarrow Y是\textcolor{orange}{\underline{\textbf{双射}}}函数)$
>**证明过程**
>$$先证 \quad \textcolor{orange}{\underline{\textbf{定义域、陪域}}}相等$$
>$$\begin{eqnarray}
>&f \textcolor{pink}{\underline{\textbf{双射}}}& \quad 故f^{-1}存在\quad (f^{-1}:Y \rightarrow X)\\ \\
>&函数复合& \quad f^{-1} \circ f : X \rightarrow X\\ \\
>&恒等函数& \quad I_{X}:X \rightarrow X\\ \\
>&综上& \quad 证毕!
\end{eqnarray}$$
$$\\ \\ $$
>$$后证 \quad \textcolor{orange}{\underline{\textbf{对应关系}}}相等$$
>$$\begin{eqnarray}
&f \textcolor{pink}{\underline{\textbf{双射}}}& \quad \forall \ x \in X \ , \ \exists \ y \in Y \quad S.t. \quad y=f(x)\\ \\
&f^{-1}存在& \quad f^{-1}(y)=f^{-1}(f(x))=x\\ \\
&\iff& \quad f^{-1} \circ f(x)=f^{-1}(f(x))=f^{-1}(y)=x=I_{X}(x)\\ \\
&综上& \quad f^{-1} \circ f = I_{X}\\ \\
&\iff& \quad 证毕!
>\end{eqnarray}$$

>[!tip] $g \circ f =I_{X}\quad且\quad f \circ g=I_{Y} \quad \Rightarrow \quad g=f^{-1}$
>**证明过程**
>$$先证 \quad f、g \textcolor{orange}{\underline{\textbf{都可逆}}}$$
>$$\\ \\ $$
>$$\begin{eqnarray}
>&I_{X}是\textcolor{pink}{\underline{\textbf{双射的}}}& \quad g \circ f 是\textcolor{orange}{\underline{\textbf{双射的}}}\\ \\
>&函数复合性质& \quad f是\textcolor{orange}{\underline{\textbf{单射的}}} \quad g是\textcolor{orange}{\underline{\textbf{满射的}}}\\ \\
>&同理& \quad f是\textcolor{orange}{\underline{\textbf{满射的}}} \quad g是\textcolor{orange}{\underline{\textbf{单射的}}}\\ \\
>&综上& \quad f、g是\textcolor{orange}{\underline{\textbf{双射的}}}\\ \\
>&\iff& \quad f、g都\textcolor{red}{\underline{\textbf{存在}}} \quad 证毕!
\end{eqnarray}$$
$$\\ $$
$$再证 \quad f、g \textcolor{pink}{\underline{\textbf{定义域、陪域}}}相等\\ \\ $$
$$显然成立!$$
$$\\ $$
$$最后证\quad \textcolor{pink}{\underline{\textbf{对应规律}}}相等$$
> $$\begin{eqnarray}
&& \quad \forall \ y \in Y \quad f^{-1}(y)=f^{-1}(I_{Y}(y))=f^{-1}(f(g(y)))=f^{-1}f(g(y))=I_{X}(g(y))=g(y)\\ \\
&\iff& \quad 证毕!
\end{eqnarray}$$