# 条件   

$$\begin{eqnarray}
条件: \quad
&①& \quad \textcolor{pink}{\underline{\textbf{无限集}}}M\\
\end{eqnarray}$$
# 证明   


$$\exists \ M的\textcolor{orange}{\underline{\textbf{真子集}}} \quad S.t. \quad  \textcolor{orange}{\underline{\textbf{真子集}}} \ \sim \ M$$
# Proof   

根据[[集合A与集合B等势]]的定义 , 只需找到

$$\tag{1}M的\textcolor{orange}{\underline{\textbf{真子集}}}$$
并且找到
$$\tag{2}\textcolor{pink}{\underline{\textbf{双射}}}f: \quad M的\textcolor{orange}{\underline{\textbf{真子集}}} \rightarrow M$$
只需令

$$\tag{1}M的\textcolor{orange}{\underline{\textbf{真子集}}}=M-\{\ a_{1}\ \}$$
首先 , 因为

$$M是\textcolor{pink}{\underline{\textbf{无限集}}}$$
根据[[定理4-5.2]]得

$$A是\textcolor{red}{\underline{\textbf{可数}}}的 \ \ 且\ \  A \subseteq M$$
然后 , 根据[[定理4-5.1]]得

$$A=\{\  a_{1} \ , \ \cdots \ , \ a_{n} \ , \ \cdots\ \}$$
不妨令

$$M=\begin{Bmatrix}
a_{1} \ , \ \cdots \ , \ a_{n} \ , \ \cdots \\
b_{1} \ , \ \cdots \ , \ b_{n} \ , \ \cdots 
\end{Bmatrix}=A+B$$
那么

$$B=M-A=\{\ b_{1} \ , \ \cdots \ , \ b_{n} \ , \ \cdots \ \}$$

首先 , 我们找到了

$$\tag{1}M的\textcolor{orange}{\underline{\textbf{真子集}}}=M-\{\ a_{1} \ \}=\begin{Bmatrix}
\sharp \ , \ \cdots \ , \ a_{n} \ , \ \cdots \\
b_{1} \ , \ \cdots \ , \ b_{n} \ , \ \cdots 
\end{Bmatrix}$$
然后 , 我们找到了

$$\tag{2}\textcolor{pink}{\underline{\textbf{双射}}}f: \quad M- \{\ a_{1}\ \} \rightarrow M$$
$$\quad \Updownarrow \quad$$
$$\tag{2}\left\{\begin{matrix}
\ f(a_{i})=a_{i+1} \quad i \in \mathbb{N}_{+}\\ 
f(b_{i})=b_{i} \quad i \in \mathbb{N}_{+}
\end{matrix}\right.$$
综上

$$\qquad QED\ !$$