## 例子 ：
$$证明(P \wedge (P \rightarrow Q)) \rightarrow Q为重言式$$
### 法1(列真值表法) :

$$即证明合式公式(P \wedge (P \rightarrow Q)) \rightarrow Q恒为T$$

列真值表得 ：
![[Pasted image 20240312162852.png]]

### 法2(等价公式变换法([[置换定律]])) ：
$\begin{eqnarray}
(P \wedge (P \rightarrow Q)) \rightarrow Q 
&=& (P \wedge (\neg P \vee Q))\rightarrow Q \\
&=& ((P \wedge \neg P)\vee (P \wedge Q))  \rightarrow Q \\
&=& (F \vee (P \wedge Q)) \rightarrow Q \\
&=&(P \wedge Q) \rightarrow Q \\ 
&=& \neg(P \wedge Q) \vee Q\\
&=& (\neg P \vee \neg Q) \vee Q \\ 
&=& \neg P \vee (\neg Q \vee Q)\\
&=& \neg P \vee T\\
&=& T
\end{eqnarray}$