>[!example] **枚举法**
>$$f:X \rightarrow Y \qquad g: Y \rightarrow Z$$
>$$X=\{1,2,3\} \quad Y=\{1,2,3,4\} \quad Z=\{1,2,3,4,5\}$$
>$$假设\qquad f=\{<1,2>,<2,4>,<3,1>\}\quad g=\{<1,3>,<2,5>,<3,2>,<4,1>\}$$
>$$g \circ f =\{<1,5>,<2,1>,<3,3>\}\quad(X \rightarrow Z)$$

>[!summary] **有向图法**
>$$f:X \rightarrow Y \qquad g: Y \rightarrow Z$$
>$$X=\{1,2,3\} \quad Y=\{1,2,3,4\} \quad Z=\{1,2,3,4,5\}$$
>$$假设\qquad f=\{<1,2>,<2,4>,<3,1>\}\quad g=\{<1,3>,<2,5>,<3,2>,<4,1>\}$$
>![[Pasted image 20240528142646.png]]

>[!tip] **谓词公式法**
>$$f、g是\mathbb{R}上的函数$$
>$$f=\{<x,y>|x,y \in R \wedge y =3x+1\}$$
>$$g=\{<x,y>|x,y \in R \wedge y =x^{2}+x\}$$
>$$\begin{eqnarray}
>g \circ f&=& \quad (3x+1)^{2}+(3x+1)\\
>f \circ g&=& \quad 3(x^{2}+x)+1\\
>f \circ f&=& \quad 3(3x+1)+1\\
>g \circ g&=& \quad (x^{2}+x)^{2}+(x^{2}+x)  
\end{eqnarray}$$

>[!check] **注释**
>$$函数复合运算\textcolor{orange}{\underline{\textbf{不满足交换律}}}$$