$$\begin{eqnarray}
条件: \quad
&①& \quad f:X \rightarrow Y\\
&②& \quad g:Y \rightarrow Z
\end{eqnarray}$$
$$\begin{eqnarray}
定理: \quad
&①& \quad if \quad f、g是\textcolor{orange}{\underline{\textbf{满射的}}} \quad \Rightarrow \quad g \circ f 是 \textcolor{red}{\underline{\textbf{满射的}}}\\
&②& \quad if \quad f、g是\textcolor{orange}{\underline{\textbf{单射的}}} \quad \Rightarrow \quad g \circ f 是 \textcolor{red}{\underline{\textbf{单射的}}}\\
&③& \quad if \quad f、g是\textcolor{orange}{\underline{\textbf{双射的}}} \quad \Rightarrow \quad g \circ f 是 \textcolor{red}{\underline{\textbf{双射的}}}\\
\end{eqnarray}$$
>[!info] **证明过程1**
>$$\begin{eqnarray}
>&g \circ f : X \rightarrow Z& \quad \forall \ z \in Z\\ \\
>&g是\textcolor{orange}{\underline{\textbf{满射的}}}& \quad \exists \ y \in Y \quad S.t. \quad z=g(y)\\ \\
>&f是\textcolor{orange}{\underline{\textbf{满射的}}}& \quad \exists \ x \in X 
>\quad S.t. \quad y=f(x)\\ \\
>&综上& \quad \forall \ z \in Z \quad \exists \ x \in X \quad S.t. \quad z=g(f(x))=g \circ f (x)\\ \\
>&\iff& g \circ f 是\textcolor{orange}{\underline{\textbf{满射的}}}\quad 证毕!
\end{eqnarray}$$

>[!hint] **证明过程2**
>$$\begin{eqnarray}
>&g \circ f :X \rightarrow Z& \quad \forall \ z_{1}、z_{2} \in Z\ 且\ z_{1} \neq z_{2}\\ \\
>&g是\textcolor{orange}{\underline{\textbf{单射的}}}& \quad \exists \ y_{1}、y_{2} \in Y \quad S.t. \quad z_{i}=g(y_{i}) \quad (y_{1} \neq y_{2})\\ \\\
>&f是\textcolor{orange}{\underline{\textbf{单射的}}}& \quad \exists \ x_{1}、
>x_{2} \in X \quad S.t. \quad y_{i}=f(x_{i}) \quad (x_{1} \neq x_{2})\\ \\
>&综上& \quad \forall \ z_{1} \neq z_{2} \in Z \quad \exists \ x_{1}\neq x_{2} \in X \quad S.t. \quad z_{i}=g(f(x_{i})) \quad (x_{1} \neq x_{2})\\ \\
>&\iff& \quad g \circ f 是\textcolor{orange}{\underline{\textbf{单射的}}} \quad 证毕!
\end{eqnarray}$$