# 条件

$$\begin{eqnarray}
条件: \quad
&①& \quad G是\textcolor{pink}{\underline{\textbf{无向图}}} 
\end{eqnarray}$$
# 证明

$$\begin{eqnarray}
if:\quad
&①& \quad n  \geqslant 11 \\
\end{eqnarray}$$
$$\quad \Downarrow \quad $$
$$G  \ \ 或 \ \ \bar{G}是 \textcolor{orange}{\underline{\textbf{非平面图}}}$$

# Proof

$$\textcolor{red}{\underline{\textbf{反证法}}}$$
假设

$$G \ \ 与\ \ \bar{G} \textcolor{red}{\underline{\textbf{都是}}} \textcolor{orange}{\underline{\textbf{平面图}}}$$
只需证明
$$n <11$$
下面进行证明 :

假设

$$|V(G)|=n \qquad |V(\bar{G})|=n^{'}$$
$$|E(G)|=e \qquad |E(\bar{G})|=e^{'}$$
$$|R(G)|=r \qquad |R(\bar{G})|=r^{'}$$
由于

$$G+ \bar{G}= K_{n}$$
因此


$$\tag{核心手法}e+ e^{'} = C_{n}^{2}= \frac{n(n-1)}{2}$$
$$\tag{核心手法}n=n^{'}$$
因为

$$G \ \ 与\ \ \bar{G}都是 \textcolor{orange}{\underline{\textbf{平面图}}}$$
由"$\textcolor{orange}{\underline{\textbf{简单平面图}}}的\textcolor{orange}{\underline{\textbf{性质}}}$"得

$$e  \leqslant 3n-6$$
$$e^{'}  \leqslant 3n^{'}-6$$
相加得

$$\frac{n(n-1)}{2}=e+e^{'}  \leqslant 3(n+n^{'})-12=6n-12$$
$$\quad \Downarrow \quad $$
$$\frac{n(n-1)}{2}  \leqslant 6n-12$$
$$\quad \Downarrow \quad $$
$$n(n-1)  \leqslant 12n -24$$
$$\quad \Downarrow \quad $$
$$n^{2} -n  \leqslant 12n -24$$
$$\quad \Downarrow \quad $$
$$n^{2} -13n +24  \leqslant 0$$
$$\quad \Downarrow \quad $$
$$ \frac{13- \sqrt{73}}{2}  \leqslant n  \leqslant \frac{13+\sqrt{73}}{2}  < \frac{13+9}{2}= \frac{22}{2} =11 \quad 矛盾!$$
$$\quad \Downarrow \quad $$
$$\qquad QED\ !$$
