$$若A(P_{1},P_{2},\cdots,P_{n})是一个只含有 \neg \ , \vee \ , \wedge的命题公式$$

$$则 \neg A(P_{1},P_{2},\cdots, P_{n}) \Leftrightarrow A^{*}(\neg P_{1}, \neg P_{2},\cdots, \neg P_{n})$$

## 推论 ：
$$ A(\neg P_{1} , \neg P_{2} , \cdots , \neg P_{n}) \Leftrightarrow \neg A^{*}(P_{1},P_{2},\cdots,P_{n}) $$

## 例子(利用对偶式定理改写命题公式) ：
$$改写\neg( ((P \wedge Q)\vee (P \wedge \neg Q))\vee R)$$


$$令A=((P \wedge Q)\vee(P \wedge \neg Q)) \vee R$$
由对偶式定理得 :
$$A^{*}=((P \vee Q) \wedge (P \vee \neg Q)) \wedge R$$
故 ：
$$A^{*}(\neg)=((\neg P \vee \neg Q)\wedge(\neg P \vee Q))\wedge \neg R$$

进而得到 ：
$$ \neg A=A^{*}(\neg)=((\neg P \vee \neg Q)\wedge(\neg P \vee Q))\wedge \neg R$$
